compiler/bootstrap/translation/decode64ProgScript.sml
@@ -1,0 +1,204 @@
+(*
+  Translate the compiler's state decoder.
+*)
+open preamble
+     num_list_enc_decTheory num_tree_enc_decTheory backend_enc_decTheory
+     x64ProgTheory ml_translatorLib ml_translatorTheory
+
+val _ = new_theory "decode64Prog"
+
+val _ = translation_extends "x64Prog";
+
+val _ = ml_translatorLib.ml_prog_update (ml_progLib.open_module "decode64Prog");
+
+(* translator setup *)
+
+val RW = REWRITE_RULE
+val RW1 = ONCE_REWRITE_RULE
+fun list_dest f tm =
+  let val (x,y) = f tm in list_dest f x @ list_dest f y end
+  handle HOL_ERR _ => [tm];
+val dest_fun_type = dom_rng
+val mk_fun_type = curry op -->;
+fun list_mk_fun_type [ty] = ty
+  | list_mk_fun_type (ty1::tys) =
+      mk_fun_type ty1 (list_mk_fun_type tys)
+  | list_mk_fun_type _ = fail()
+
+val _ = add_preferred_thy "-";
+val _ = add_preferred_thy "termination";
+
+Theorem NOT_NIL_AND_LEMMA:
+   (b <> [] /\ x) = if b = [] then F else x
+Proof
+  Cases_on `b` THEN FULL_SIMP_TAC std_ss []
+QED
+
+val extra_preprocessing = ref [MEMBER_INTRO,MAP];
+
+fun def_of_const tm = let
+  val res = dest_thy_const tm handle HOL_ERR _ =>
+              failwith ("Unable to translate: " ^ term_to_string tm)
+  val name = (#Name res)
+  fun def_from_thy thy name =
+    DB.fetch thy (name ^ "_pmatch") handle HOL_ERR _ =>
+    DB.fetch thy (name ^ "_def") handle HOL_ERR _ =>
+    DB.fetch thy (name ^ "_DEF") handle HOL_ERR _ =>
+    DB.fetch thy name
+  val def = def_from_thy "termination" name handle HOL_ERR _ =>
+            def_from_thy (#Thy res) name handle HOL_ERR _ =>
+            failwith ("Unable to find definition of " ^ name)
+  val def = def |> RW (!extra_preprocessing)
+                |> CONV_RULE (DEPTH_CONV BETA_CONV)
+                |> SIMP_RULE bool_ss [IN_INSERT,NOT_IN_EMPTY]
+                |> REWRITE_RULE [NOT_NIL_AND_LEMMA]
+  in def end
+
+val _ = (find_def_for_const := def_of_const);
+
+(* --- *)
+
+val res = translate dec_next_def;
+val res = translate chars_to_nums_def;
+
+val res = translate const_dec_def;
+val res = translate unit_dec_def;
+val res = translate num_dec_def;
+val res = translate num_list_enc_decTheory.list_dec'_def;
+val res = translate list_dec_def;
+val res = translate bool_dec_def;
+val res = translate int_dec_def;
+val _ = next_ml_names := ["word8_dec"];
+val res = translate (word_dec_def |> INST_TYPE [alpha|->“:8”]);
+val _ = next_ml_names := ["word64_dec"];
+val res = translate (word_dec_def |> INST_TYPE [alpha|->“:64”]);
+val res = translate char_dec_def;
+val res = translate num_list_enc_decTheory.mlstring_dec_def;
+val res = translate prod_dec_def;
+val res = translate option_dec_def;
+val res = translate sum_dec_def;
+val res = translate spt_dec'_def;
+val res = translate spt_dec''_def;
+val res = translate spt_dec_def;
+val res = translate namespace_dec'_def;
+val res = translate namespace_dec_def;
+
+(* --- *)
+
+val res = translate num_tree_dec'_def;
+val res = translate num_tree_dec_def;
+val res = translate nth_def;
+val res = translate int_dec'_def;
+val res = translate bool_dec'_def;
+val res = translate chr_dec'_def;
+val res = translate list_dec'_def;
+val res = translate pair_dec'_def;
+val res = translate option_dec'_def;
+
+(* --- *)
+
+val _ = ml_translatorLib.use_string_type false;
+val res = translate (tra_dec'_def |> DefnBase.one_line_ify NONE);
+val res = translate safe_chr_list_def;
+val res = translate list_chr_dec'_def;
+val _ = ml_translatorLib.use_string_type true;
+val res = translate string_dec_def;
+val res = translate next_indices_dec_def;
+val res = translate flat_pattern_config_dec_def;
+val res = translate namespace_dec'_def;
+val res = translate namespace_dec_def;
+val res = translate (var_name_dec'_def |> REWRITE_RULE [string_dec'_intro]);
+val res = translate var_name_dec_def;
+val res = translate environment_dec_def;
+val res = translate environment_store_dec_def;
+val res = translate source_to_flat_config_dec_def;
+val _ = ml_translatorLib.use_string_type false;
+
+val res = translate data_to_word_config_dec_def;
+val res = translate word_to_word_config_dec_def;
+val res = translate (word_to_stack_config_dec_def |> INST_TYPE [alpha|->“:64”]);
+val res = translate stack_to_lab_config_dec_def;
+
+val res = translate (mlstring_dec'_def |> REWRITE_RULE [GSYM mlstringTheory.implode_def]);
+val res = translate tap_config_dec'_def;
+val res = translate tap_config_dec_def;
+
+val res = translate (closLang_op_dec'_def |> DefnBase.one_line_ify NONE);
+
+Theorem list_dec'_eq_MAP:
+  ∀f t. list_dec' f t = MAP f (list_dec' I t)
+Proof
+  Cases_on ‘t’ \\ fs [list_dec'_def]
+QED
+
+val def = bvl_exp_dec'_def |> DefnBase.one_line_ify NONE
+          |> ONCE_REWRITE_RULE [list_dec'_eq_MAP]
+val res = translate def;
+
+val res = translate bvl_to_bvi_config_dec_def;
+
+Theorem pair_dec'_eq:
+  pair_dec' d1 d2 = λt. (d1 (nth 0 (list_dec' I t)), d2 (nth 1 (list_dec' I t)))
+Proof
+  fs [FUN_EQ_THM,FORALL_PROD]
+  \\ Cases \\ fs [pair_dec'_def,list_dec'_def]
+QED
+
+val def = closLang_exp_dec'_def |> DefnBase.one_line_ify NONE
+          |> ONCE_REWRITE_RULE [list_dec'_eq_MAP]
+          |> ONCE_REWRITE_RULE [pair_dec'_eq]
+          |> CONV_RULE (DEPTH_CONV BETA_CONV)
+val res = translate_no_ind def;
+
+val ind_lemma = Q.prove(
+  `^(first is_forall (hyp res))`,
+  rpt gen_tac
+  \\ rpt (disch_then strip_assume_tac)
+  \\ match_mp_tac (latest_ind ())
+  \\ rpt strip_tac
+  \\ last_x_assum irule
+  \\ rewrite_tac [num_tree_11]
+  \\ rpt gen_tac \\ strip_tac
+  \\ rpt var_eq_tac
+  \\ gen_tac \\ disch_then (assume_tac o SYM)
+  \\ Cases_on ‘x6 = 0’ \\ asm_rewrite_tac [] THEN1 (gvs [ADD1])
+  \\ ‘n ≠ 1 ∧ n ≠ 0’ by decide_tac
+  \\ Cases_on ‘x6 = 1’ \\ asm_rewrite_tac [] THEN1 (gvs [ADD1])
+  \\ ‘n ≠ 2’ by decide_tac
+  \\ Cases_on ‘n = 3’ \\ asm_rewrite_tac [] THEN1 (gvs [ADD1])
+  \\ Cases_on ‘n = 4’ \\ asm_rewrite_tac [] THEN1 (gvs [ADD1])
+  \\ Cases_on ‘n = 5’ \\ asm_rewrite_tac [] THEN1 (gvs [ADD1])
+  \\ Cases_on ‘n = 6’ \\ asm_rewrite_tac [] THEN1 (gvs [ADD1])
+  \\ Cases_on ‘n = 7’ \\ asm_rewrite_tac [] THEN1 (gvs [ADD1])
+  \\ Cases_on ‘n = 8’ \\ asm_rewrite_tac [] THEN1 (gvs [ADD1])
+  \\ Cases_on ‘n = 9’ \\ asm_rewrite_tac []
+  \\ rpt var_eq_tac \\ gvs [ADD1])
+  |> update_precondition;
+
+val def = val_approx_dec'_def |> DefnBase.one_line_ify NONE
+          |> ONCE_REWRITE_RULE [list_dec'_eq_MAP]
+val res = translate def;
+
+val def = clos_to_bvl_config_dec_def
+val res = translate def;
+
+val _ = ml_translatorLib.use_string_type true;
+val def = lab_to_target_config_dec_def |> INST_TYPE [alpha|->“:64”]
+          |> REWRITE_RULE [GSYM string_dec_thm]
+val res = translate def;
+val _ = ml_translatorLib.use_string_type false;
+
+val _ = register_type “:64 backend$config”;
+
+val def = config_dec_def |> INST_TYPE [alpha|->“:64”]
+val res = translate def;
+
+val res = translate (decode_backend_config_def |> INST_TYPE [alpha|->“:64”]);
+
+val () = Feedback.set_trace "TheoryPP.include_docs" 0;
+
+val _ = ml_translatorLib.ml_prog_update (ml_progLib.close_module NONE);
+
+val _ = (ml_translatorLib.clean_on_exit := true);
+
+val _ = export_theory();
